\documentclass[10pt,a4paper]{article}
\usepackage[utf8]{inputenc}
\usepackage{amsmath}
\usepackage{amsfonts}
\usepackage{amssymb}
\begin{document}


Next we note that $\lambda^{-1}$ is homogeneous of degree $-\gamma$ so \
$\partial^\alpha_\xi \partial^\beta_\eta \lambda^{-1}$ 
is homogeneous of degree $-\gamma -|\alpha + \beta|$. 
That is $\partial^\alpha_\xi 
\partial^\beta_\eta 
\lambda^{-1} (r \xi, r \eta) = 
r^{-\gamma -|\alpha+\beta|}\partial^\alpha_\xi \partial^\beta_\eta \gamma^{-1}(\xi,\eta)$ for any $r>0$. 
By letting $r = (\abs{\xi} + \abs{\eta})^{-1}$ we obtain 

\bibliography{NaiboThomsonBiblio}
\end{document}